SystemFD/Metatheory/Preservation.lean
@@ -1,0 +1,169 @@
+import SystemFD.Term
+import SystemFD.Term.Definition
+import SystemFD.Judgment
+import SystemFD.Ctx
+import SystemFD.Reduction
+import SystemFD.Metatheory.Weaken
+import SystemFD.Metatheory.Substitution
+
+theorem preservation_inst_lemma :
+  Γ ⊢ t : A ->
+  t.neutral_form = .some (x, sp) ->
+  Γ.is_openm x' ->
+  ixs = instance_indices' Γ 0 x' [] ->
+  w ∈ get_instances Γ ixs ->
+  Γ ⊢ w.apply_spine sp : A
+:= by sorry
+
+theorem preservation_letterm_lemma :
+  Γ ⊢ a : A ->
+  a.neutral_form = some (x, sp) ->
+  Frame.term T t = Γ d@ x ->
+  Γ ⊢ t.apply_spine sp : A
+:= by sorry
+
+theorem preservation_prefix_match_lemma {p s t : Term} :
+  Γ ⊢ p : A ->
+  Γ ⊢ s : R ->
+  Γ ⊢ t : B ->
+  PrefixTypeMatch Γ A B T ->
+  some ξ = prefix_equal sp sp' ->
+  some (x, sp) = p.neutral_form ->
+  some (x, sp') = s.neutral_form ->
+  Γ ⊢ t.apply_spine ξ : T
+:= by
+intro j1 j2 j3 j4 j5 j6 j7
+induction j4 generalizing x sp sp' p s ξ t
+case _ => sorry
+case _ Γ A B V T h ih =>
+
+  sorry
+case _ => sorry
+
+@[simp]
+abbrev PreservationStepType (Γ : Ctx Term) : (v : JudgmentVariant) -> JudgmentArgs v -> Prop
+| .prf => λ (t, A) => ∀ {ℓ t'}, Red Γ t ℓ -> t' ∈ ℓ -> Γ ⊢ t' : A
+| .wf => λ () => True
+
+theorem preservation_step : Judgment v Γ ix -> PreservationStepType Γ v ix := by
+intro j
+induction j <;> simp at *
+all_goals (intro ℓ t' r rin)
+any_goals (solve | cases r <;> simp at *)
+case _ j1 j2 j3 j4 ih1 ih2 ih3 ih4 =>
+  cases r <;> simp at *; subst rin
+  have lem := beta_term j3 j2; simp at lem
+  apply lem
+case _ wf j _ =>
+  cases r <;> try simp at *
+  case _ x sp ixs ℓ i1 i2 i3 i4 i5 =>
+    cases i5; case _ e1 e2 =>
+      subst e1; subst e2
+      unfold Frame.is_openm at i1; split at i1 <;> simp at *
+      case _ f T h =>
+        rw [h] at j; unfold Frame.get_type at j; simp at j
+        subst i4; subst j; subst i3
+        sorry
+  case _ A x sp t h1 h2 =>
+    cases h2; case _ h2 h3 =>
+      subst h2; subst h3; unfold Term.apply_spine at rin
+      subst rin; rw [<-h1] at j; unfold Frame.get_type at j; simp at j
+      subst j
+      sorry
+case appk =>
+  cases r
+  case _ =>
+    sorry
+  case _ =>
+    sorry
+case ite j1 j2 j3 j4 j5 j6 j7 j8 j9 j10 ih1 ih2 ih3 ih4 ih5 ih6 =>
+  cases r <;> try simp at *
+  case _ x sp sp' ξ h1 h2 h3 h4 =>
+    subst rin
+    apply preservation_prefix_match_lemma j1 j2 j4 j8 h1 h3 h4
+  case _ => subst rin; apply j10
+  case _ ℓ' r h =>
+    subst h; simp at rin
+    cases rin; case _ w h =>
+    cases h; case _ h1 h2 =>
+      subst h2; replace ih2 := ih2 r h1
+      apply Judgment.ite j1 ih2 j3 j4 j5 j6 j7 j8 j9 j10
+case guard j1 j2 j3 j4 j5 j6 j7 j8 j9 ih1 ih2 ih3 ih4 ih5 =>
+  cases r <;> try simp at *
+  case _ x sp sp' ξ h1 h2 h3 =>
+    subst rin
+    apply preservation_prefix_match_lemma j1 j2 j4 j8 h1 h2 h3
+  case _ ℓ' r h =>
+    subst h; simp at rin
+    cases rin; case _ w h =>
+    cases h; case _ h1 h2 =>
+      subst h2; replace ih2 := ih2 r h1
+      apply Judgment.guard j1 ih2 j3 j4 j5 j6 j7 j8 j9
+case _ j1 j2 j3 ih1 ih2 =>
+  cases r
+  case _ =>
+    simp at rin; subst rin
+    cases j1; case _ j4 j5 j6 =>
+      have lem := beta_type j6 j2
+      subst j3; apply lem
+  case _ x sp ixs ℓ' i1 i2 i3 i4 i5 =>
+    simp at i4; replace i4 := Eq.symm i4
+    rw [Option.bind_eq_some] at i4; simp at i4
+    cases i4; case _ x' i4 =>
+    cases i4; case _ sp' i4 =>
+    cases i4; case _ h1 h2 =>
+    cases h2; case _ h2 h3 =>
+      subst h2; subst h3; subst i5
+      simp at rin; cases rin; case _ w rin =>
+      cases rin; case _ q1 q2 =>
+        subst q2; subst i3
+        have lem := preservation_inst_lemma j1 h1 i1 i2 q1
+        rw [Term.apply_spine_peel_term]; constructor
+        apply lem; apply j2; apply j3
+  case _ T x sp t i1 i2 =>
+    simp at i2; replace i2 := Eq.symm i2
+    rw [Option.bind_eq_some] at i2; simp at i2
+    cases i2; case _ x' i2 =>
+    cases i2; case _ sp' i2 =>
+    cases i2; case _ h1 h2 =>
+    cases h2; case _ h2 h3 =>
+      subst h2; subst h3; simp at rin; subst rin
+      have lem := preservation_letterm_lemma j1 h1 i1
+      rw [Term.apply_spine_peel_term]; constructor
+      apply lem; apply j2; apply j3
+  case _ ℓ' r h =>
+    subst h; simp at rin
+    cases rin; case _ f' h =>
+    cases h; case _ h1 h2 =>
+      subst h2; constructor
+      apply ih1 r h1; apply j2; apply j3
+case appt => sorry
+case _ j1 j2 ih1 ih2 =>
+  cases r <;> try simp at *
+  case _ =>
+    subst rin; cases j2; case _ =>
+      apply j1
+  case _ ℓ' r' h =>
+    subst h; simp at rin
+    cases rin; case _ z h =>
+    cases h; case _ h1 h2 =>
+      subst h2; constructor
+      apply j1; apply ih2 r' h1
+case _ j ih =>
+  cases r <;> try simp at *
+  case _ =>
+    subst rin; cases j; case _ j1 j2 =>
+      constructor; apply j1; apply j2
+  case _ ℓ' r' h =>
+    subst h; simp at rin
+    cases rin; case _ z h =>
+    cases h; case _ h1 h2 =>
+      subst h2; constructor
+      apply ih r' h1
+case seq => sorry
+case _ => sorry
+case _ => sorry
+case _ => sorry
+case _ => sorry
+case _ => sorry
+case _ => sorry
