SystemFD/Reduction.lean
@@ -52,7 +52,7 @@ inductive Red : Ctx Term -> Term -> List Term -> Prop where
 ----------------------------------------------------------------
 | inst :
   .some (x, sp) = Term.neutral_form h ->
-  Term.is_openmethod Γ x ->
+  Γ.is_openm x ->
   indices = instance_indices' Γ 0 x [] -> -- searches for the instances of open method x
   -- indices.length > 0 ->
   tl = get_instances Γ indices -> -- weakens the instances
